Semantic/Capybara/Syntax/Ty.lean
@@ -44,10 +44,9 @@ inductive Ty : TySort -> Sig -> Type where
 -- capturing types
 | top : Ty .capt s
 | tvar : BVar s .tvar -> Ty .capt s
-| arrow : Ty .capt s -> CaptureSet s -> Ty .exi (s,x) -> Ty .capt s
+| arrow : Ty .capt (s,C) -> CaptureSet s -> Ty .exi (s,x) -> Ty .capt s
 | poly : Ty .capt s -> CaptureSet s -> Ty .exi (s,X) -> Ty .capt s
 | cpoly : CaptureBound s -> CaptureSet s -> Ty .exi (s,C) -> Ty .capt s
-| modal : CaptureSet s -> SepCtx s -> Ty .exi s -> Ty .capt s
 | cap : CaptureSet s -> Ty .capt s
 | cell : CaptureSet s -> Ty .capt s
 | reader : CaptureSet s -> Ty .capt s
@@ -61,10 +60,9 @@ inductive Ty : TySort -> Sig -> Type where
 def Ty.rename : Ty sort s1 -> Rename s1 s2 -> Ty sort s2
 | .top, _ => .top
 | .tvar x, f => .tvar (f.var x)
-| .arrow T1 cs T2, f => .arrow (T1.rename f) (cs.rename f) (T2.rename (f.lift))
+| .arrow T1 cs T2, f => .arrow (T1.rename (f.lift)) (cs.rename f) (T2.rename (f.lift))
 | .poly T1 cs T2, f => .poly (T1.rename f) (cs.rename f) (T2.rename (f.lift))
 | .cpoly cb cs T, f => .cpoly (cb.rename f) (cs.rename f) (T.rename (f.lift))
-| .modal cs Ψ T, f => .modal (cs.rename f) (Ψ.rename f) (T.rename f)
 | .unit, _ => .unit
 | .cap cs, f => .cap (cs.rename f)
 | .bool, _ => .bool
@@ -80,17 +78,14 @@ def Ty.rename_id {T : Ty sort s} : T.rename (Rename.id) = T := by
   | tvar x =>
     simp only [Ty.rename, Rename.id]
   | arrow T1 cs T2 ih1 ih2 =>
-    simp only [Ty.rename, Rename.lift_id, CaptureSet.rename_id, ih1]
-    exact congrArg (Ty.arrow T1 cs) ih2
+    simp only [Ty.rename, Rename.lift_id, CaptureSet.rename_id]
+    congr 1
   | poly T1 cs T2 ih1 ih2 =>
     simp only [Ty.rename, Rename.lift_id, CaptureSet.rename_id, ih1]
     exact congrArg (Ty.poly T1 cs) ih2
   | cpoly cb cs T ih =>
     simp only [Ty.rename, Rename.lift_id, CaptureBound.rename_id, CaptureSet.rename_id]
     exact congrArg (Ty.cpoly cb cs) ih
-  | modal cs Ψ T ih =>
-    simp only [Ty.rename, CaptureSet.rename_id, SepCtx.rename_id]
-    exact congrArg (Ty.modal cs Ψ) ih
   | cap cs =>
     simp only [Ty.rename, CaptureSet.rename_id]
   | cell cs =>
@@ -114,9 +109,10 @@ theorem Ty.rename_comp {T : Ty sort s1} {f : Rename s1 s2} {g : Rename s2 s3} :
   | tvar x =>
     simp only [Ty.rename, Rename.comp]
   | arrow T1 cs T2 ih1 ih2 =>
-    simpa only [Ty.rename, CaptureSet.rename_comp, Rename.lift_comp, ih1] using
-      congrArg (Ty.arrow (T1.rename (f.comp g)) (cs.rename (f.comp g)))
-        (ih2 (f := f.lift) (g := g.lift))
+    simp only [Ty.rename, CaptureSet.rename_comp, Rename.lift_comp]
+    congr 1
+    · exact ih1 (f := f.lift) (g := g.lift)
+    · exact ih2 (f := f.lift) (g := g.lift)
   | poly T1 cs T2 ih1 ih2 =>
     simpa only [Ty.rename, CaptureSet.rename_comp, Rename.lift_comp, ih1] using
       congrArg (Ty.poly (T1.rename (f.comp g)) (cs.rename (f.comp g)))
@@ -125,10 +121,6 @@ theorem Ty.rename_comp {T : Ty sort s1} {f : Rename s1 s2} {g : Rename s2 s3} :
     simpa only [Ty.rename, CaptureBound.rename_comp, CaptureSet.rename_comp, Rename.lift_comp] using
       congrArg (Ty.cpoly (cb.rename (f.comp g)) (cs.rename (f.comp g)))
         (ih (f := f.lift) (g := g.lift))
-  | modal cs Ψ T ih =>
-    simpa only [Ty.rename, CaptureSet.rename_comp, SepCtx.rename_comp] using
-      congrArg (Ty.modal (cs.rename (f.comp g)) (Ψ.rename (f.comp g)))
-        (ih (f := f) (g := g))
   | cap cs =>
     simp only [Ty.rename, CaptureSet.rename_comp]
   | cell cs =>
@@ -155,7 +147,6 @@ def Ty.captureSet : Ty .capt s -> CaptureSet s
 | .arrow _ cs _ => cs
 | .poly _ cs _ => cs
 | .cpoly _ cs _ => cs
-| .modal cs _ _ => cs
 | .cap cs => cs
 | .cell cs => cs
 | .reader cs => cs
@@ -168,7 +159,6 @@ def Ty.refineCaptureSet : Ty .capt s -> CaptureSet s -> Ty .capt s
 | .arrow T1 _ T2, cs => .arrow T1 cs T2
 | .poly T1 _ T2, cs => .poly T1 cs T2
 | .cpoly cb _ T, cs => .cpoly cb cs T
-| .modal _ Ψ T, cs => .modal cs Ψ T
 | .cap _, cs => .cap cs
 | .cell _, cs => .cell cs
 | .reader _, cs => .reader cs
@@ -191,9 +181,6 @@ inductive Ty.IsClosed : Ty sort s -> Prop where
 | cpoly :
     CaptureBound.IsClosed cb -> CaptureSet.IsClosed cs -> Ty.IsClosed T ->
     Ty.IsClosed (.cpoly cb cs T)
-| modal :
-    CaptureSet.IsClosed cs -> SepCtx.IsClosed Ψ -> Ty.IsClosed T ->
-    Ty.IsClosed (.modal cs Ψ T)
 | unit : Ty.IsClosed .unit
 | cap : CaptureSet.IsClosed cs -> Ty.IsClosed (.cap cs)
 | bool : Ty.IsClosed .bool
